wip: working on s_min owner step

fairness/lawyer/obligations/obls_termination.v
@@ -2,7 +2,7 @@ From iris.proofmode Require Import tactics.
 From iris.algebra Require Import gset gmultiset.
 From trillium.fairness Require Import locales_helpers inftraces fairness trace_len.
 From trillium.fairness.lawyer.obligations Require Import obligations_model.
-
+From stdpp Require Import relations.
 
 Ltac mss := multiset_solver. 
 
@@ -296,6 +296,10 @@ Section MultisetDefs.
       apply gmultiset_elem_of_elements.
     Qed. 
   
+    Lemma mset_map_empty:
+      mset_map ∅ = ∅. 
+    Proof using. mss. Qed. 
+  
     Lemma mset_map_disj_union (X Y: gmultiset A):
       mset_map (X ⊎ Y) = mset_map X ⊎ mset_map Y.
     Proof using.
@@ -364,23 +368,526 @@ Section MultisetDefs.
 
   End MultisetMap.
 
-  Definition mset_filter (P : A → Prop)
-    `{∀ x, Decision (P x)}
-    (g: gmultiset A): gmultiset A.
-  Admitted. 
+  Section MultisetFilter.
+    Context (P : A → Prop). 
+    Context `{∀ x, Decision (P x)}. 
 
+    Definition mset_filter (g: gmultiset A): gmultiset A :=
+      list_to_set_disj $ filter P $ elements g. 
+
+    Lemma mset_filter_spec g:
+      forall a, a ∈ mset_filter g <-> a ∈ g /\ P a.
+    Proof using.
+      intros. rewrite /mset_filter.
+      rewrite elem_of_list_to_set_disj elem_of_list_filter.
+      rewrite gmultiset_elem_of_elements. tauto.
+    Qed.
+
+    Lemma mset_filter_empty:
+      mset_filter ∅ = ∅. 
+    Proof using. mss. Qed.
+
+    Lemma mset_filter_disj_union x y:
+      mset_filter (x ⊎ y) = mset_filter x ⊎ mset_filter y.
+    Proof using.
+      rewrite /mset_filter.
+      rewrite -list_to_set_disj_app. rewrite -filter_app. 
+      apply list_to_set_disj_perm. apply filter_Permutation.
+      apply gmultiset_elements_disj_union.
+    Qed.
+
+    Lemma mset_filter_False g
+      (FALSE: forall a, a ∈ g -> ¬ P a):
+      mset_filter g = ∅.
+    Proof using.
+      destruct (decide (mset_filter g = ∅)) as [| NE]; [done| ]. 
+      apply gmultiset_choose in NE as [? IN].
+      apply mset_filter_spec in IN as [??]. set_solver.
+    Qed. 
+
+    Lemma mset_filter_singleton a:
+      mset_filter {[+ a +]} = if (decide (P a)) then {[+ a +]} else ∅.
+    Proof using.
+      rewrite /mset_filter. rewrite gmultiset_elements_singleton.
+      rewrite filter_cons !filter_nil.
+      destruct decide; mss.
+    Qed. 
+
+    Lemma mset_filter_multiplicity g (a: A):
+      multiplicity a (mset_filter g) =
+      if (decide (P a)) then multiplicity a g else 0.
+    Proof using. 
+      revert a. pattern g. apply gmultiset_ind; clear g. 
+      { intros ?. rewrite mset_filter_empty multiplicity_empty.
+        destruct decide; auto. }
+      intros x g IH a.
+      rewrite mset_filter_disj_union mset_filter_singleton.
+      rewrite !multiplicity_disj_union. rewrite multiplicity_singleton'. 
+      rewrite IH. 
+      destruct (decide (P x)), (decide (P a)); try rewrite multiplicity_singleton'.
+      - lia.
+      - rewrite decide_False; [| by intros ->]. lia.
+      - rewrite decide_False; [| by intros ->].
+        rewrite multiplicity_empty. lia.
+      - rewrite multiplicity_empty. lia.
+    Qed.
+
+    Lemma mset_filter_subseteq_mono:
+      Proper (subseteq ==> subseteq) mset_filter.
+    Proof using.
+      red. intros ????.
+      rewrite !mset_filter_multiplicity.
+      destruct decide; mss.
+    Qed. 
+
+    Lemma mset_filter_difference x y:
+      mset_filter (x ∖ y) = mset_filter x ∖ mset_filter y.
+    Proof using.
+      apply gmultiset_eq. intros a.
+      rewrite !multiplicity_difference !mset_filter_multiplicity !multiplicity_difference.
+      destruct decide; mss. 
+    Qed.
+
+    Lemma mset_filter_mul_comm g n:
+      mset_filter (n *: g) = n *: mset_filter g.
+    Proof using.
+      apply gmultiset_eq. intros ?.
+      rewrite multiplicity_scalar_mul.
+      rewrite !mset_filter_multiplicity.
+      destruct decide; try mss. 
+      by rewrite multiplicity_scalar_mul.
+    Qed. 
+
+  End MultisetFilter.
+  
 End MultisetDefs.
 
 
 Definition maximal {A C : Type} {H : ElemOf A C} (R : relation A) (x : A) (X : C) :=
   minimal (flip R) x X.
 
-
-
 Section Termination.
   Context `(OP: ObligationsParams Degree Level Locale LIM_STEPS).
   Context `{Countable Locale}. 
   Let OM := ObligationsModel OP.
+
+  Section WfSetMin.
+
+    Definition minimal_in_prop {A: Type} (R : relation A) (x : A) (P : A -> Prop) :=
+      ∀ y : A, P y → R y x → R x y. 
+
+    Context `{R: relation A}.
+    Hypothesis (SIG_WF: wf R).
+
+    Theorem sets_have_min (P: A -> Prop)
+      (NE: exists a, P a):
+      exists a, P a /\ minimal_in_prop R a P. 
+    Proof. Admitted. 
+
+  End WfSetMin.
+
+
+  Section SignalsEventuallySet.
+    Context (tr: obls_trace OP).
+
+    Context (sig_le: relation Level).
+    Hypothesis (SIG_WF: wf (strict sig_le)).
+
+    Context (lvl__def: Level). 
+
+    Definition lvl_at (sid_i: SignalId * nat): Level :=
+      let '(sid, i) := sid_i in
+      from_option (fun δ => from_option fst lvl__def (ps_sigs _ δ !! sid)) lvl__def (tr S!! i).
+
+    Require Import Coq.Program.Wf.
+    
+    Definition tr_sig_lt: relation (SignalId * nat) := MR (strict sig_le) lvl_at. 
+
+(*     wf (MR R m) *)
+(* measure_wf *)
+
+    Lemma tr_sig_lt_wf: wf tr_sig_lt.
+    Proof using SIG_WF. apply measure_wf. apply SIG_WF. Qed.
+
+    Definition never_set_after sid c := 
+      forall i, c <= i -> from_option (fun δ => from_option snd true (ps_sigs _ δ !! sid)) true (tr S!! i) = false. 
+
+    Context {set_before: SignalId -> nat}.
+
+    Definition approx_expects (k: nat) (eps: gset (@ExpectPermission Degree)) :=
+      ([^op set] ep ∈ eps, let '(sid, π, d) := ep in
+        (2 * (LIM_STEPS + 2) * set_before sid - k) *: {[+ d +]}
+      ).
+
+    Instance cmp_phase'_dec: forall (x y: Phase * Degree),
+        Decision (phase_le x.1 y.1).
+    Proof using.
+      intros [??] [??]. simpl.
+      rewrite /phase_le. solve_decision.
+    Qed. 
+
+    Local Instance cmp_phase'_dec' π0:
+      ∀ x : Phase * Degree, Decision ((λ '(π, _), phase_le π π0) x). 
+    Proof using.
+      intros [??]. simpl.
+      rewrite /phase_le. solve_decision.
+    Qed.
+
+    Local Instance cmp_phase'_dec'' π0:
+    ∀ x : SignalId * Phase * Degree, Decision ((λ '(_, π, _), phase_le π π0) x).
+    Proof using.
+      intros [[??]?]. rewrite /phase_le. solve_decision.
+    Qed. 
+
+    Let π0 := namespaces.nroot. 
+    Definition PF (π: Phase) (k: nat) (δ: ProgressState OP) :=
+      (mset_map snd ∘ (mset_filter (fun '(π_, _) => phase_le π_ π)) ∘ (ps_cps OP)) δ
+        ⊎
+      approx_expects k (filter (fun '(_, π_, _) => phase_le π_ π) (ps_eps OP δ)). 
+
+    Definition TPF (π: Phase) (i: nat): gmultiset Degree :=
+      from_option (PF π ((LIM_STEPS + 2) * i)) ∅ (tr S!! i).
+
+    Context (deg_le: relation Degree).
+
+    (* TODO: move *)
+    Lemma scalar_mul_le `{Countable K} (s: gmultiset K) m n
+      (LE: m <= n):
+      m *: s ⊆ n *: s.
+    Proof using.
+      clear -LE. 
+      apply Nat.le_sum in LE as [d ->]. multiset_solver.
+    Qed.
+
+    Lemma ms_le_exp_le m n eps
+      (LE: m <= n):
+      ms_le deg_le (approx_expects n eps) (approx_expects m eps).
+    Proof using. 
+      rewrite /approx_expects.
+      eapply big_opS_ms_le. intros [[??]?].
+      apply ms_le_sub.
+      apply scalar_mul_le. lia.
+    Qed.
+
+    Lemma approx_expects_add k eps e 
+      (FRESH: e ∉ eps):
+      let n := (2 * (LIM_STEPS + 2) * set_before (fst $ fst e) - k) in
+      approx_expects k (eps ∪ {[ e ]}) = approx_expects k eps ⊎ n *: {[+ e.2 +]}.
+    Proof using.
+      rewrite (union_comm_L _ {[ e ]}).
+      rewrite /approx_expects.
+      rewrite -leibniz_equiv_iff. 
+      rewrite big_opS_insert; auto.
+      rewrite gmultiset_op gmultiset_disj_union_comm. f_equiv.
+      destruct e as [[??]?]. done.
+    Qed.
+
+    (* TODO: move *)
+    Lemma gset_singleton_if_equiv `{Countable K} (P: K -> Prop)
+      `{forall k, Decision (P k)}:
+      forall k, filter P ({[ k ]}: gset K) = if (decide (P k)) then {[ k ]} else ∅.
+    Proof using.
+      clear -EqDecision1. 
+      intros. destruct decide; set_solver.
+    Qed.
+
+    Definition phases_incompat π1 π2 := ¬ phase_le π1 π2 /\ ¬ phase_le π2 π1. 
+
+    (* Definition loc_step_no_exp sid δ1 τ δ2 := *)
+    (*   loc_step OP δ1 τ δ2 /\ (forall π d, ¬ expects_ep OP δ1 τ δ2 sid π d). *)
+
+    Definition loc_step_no_exp_all δ1 τ δ2 :=
+      (exists π δ, burns_cp OP δ1 τ δ2 π δ) \/
+      (exists π δ δ' n, exchanges_cp OP δ1 τ δ2 π δ δ' n) \/
+      (exists l, creates_signal OP δ1 τ δ2 l) \/
+      (exists s, sets_signal OP δ1 τ δ2 s) \/
+      (exists s π δ δ', creates_ep OP δ1 τ δ2 s π δ δ').
+
+    Lemma loc_step_split δ1 τ δ2:
+      loc_step OP δ1 τ δ2 <->
+      (loc_step_no_exp_all δ1 τ δ2 \/ (exists sid π d, expects_ep OP δ1 τ δ2 sid π d)).
+    Proof using.
+      clear set_before. 
+      rewrite /loc_step_no_exp_all. split.
+      - intros [T|[T|[T|[T|[T|T]]]]]; tauto.
+      - intros [[T|[T|[T|[T|T]]]] | ?]; red; tauto.
+    Qed. 
+      
+    Lemma loc_step_no_exp_all_ms_le π__ow δ1 τ δ2 k
+      (STEP: loc_step_no_exp_all δ1 τ δ2)
+      (* (OTHER: *)
+      (*   let π := default π0 (ps_phases _ δ1 !! τ) in *)
+      (*   phases_incompat π__ow π) *)
+      :
+      ms_le deg_le (PF π__ow (S k) δ2) (PF π__ow k δ1).
+    Proof using.
+      rewrite /PF.
+      destruct STEP as [T|[T|[T|[T|T]]]]. 
+      - destruct T as (?&?&T). inversion T; subst. 
+        destruct δ1. simpl in *.
+        apply ms_le_disj_union.
+        + apply ms_le_sub. apply mset_map_sub. apply mset_filter_subseteq_mono. mss.
+        + apply ms_le_exp_le. lia.
+      - destruct T as (?&?&?&?&T). inversion T; subst. 
+        destruct δ1. simpl in *. 
+        apply ms_le_disj_union.
+        + subst new_cps0.
+          rewrite !mset_filter_disj_union mset_map_disj_union.
+          rewrite !mset_filter_difference. 
+          rewrite !mset_filter_mul_comm.
+          rewrite !mset_filter_singleton. 
+          destruct decide.
+          2: { rewrite decide_False; [| tauto].
+               rewrite multiset_difference_empty gmultiset_scalar_mul_empty.
+               rewrite mset_map_empty.
+               eapply ms_le_Proper; [reflexivity | | reflexivity].
+               mss. }
+          rewrite decide_True; [| tauto].
+          rewrite mset_map_sub_diff. 
+          2: { apply gmultiset_singleton_subseteq_l.
+               by apply mset_filter_spec. }
+          rewrite mset_map_mul !mset_map_singleton. simpl.
+          apply ms_le_exchange.
+          * admit.
+          * eapply elem_of_mset_map. eexists (_, _). split; eauto.
+            apply mset_filter_spec. split; eauto. 
+          * admit.          
+        + apply ms_le_exp_le. lia. 
+      - destruct T as (?&T). inversion T; subst.
+        destruct δ1. simpl in *.
+        apply ms_le_disj_union.
+        + apply ms_le_sub. apply mset_map_sub. mss. 
+        + apply ms_le_exp_le. lia. 
+      - destruct T as (?&T). inversion T; subst.
+        destruct δ1. simpl in *.  
+        apply ms_le_disj_union.
+        + apply ms_le_sub. apply mset_map_sub. mss. 
+        + apply ms_le_exp_le. lia. 
+      - destruct T as (?&?&?&?&T). inversion T; subst.
+        destruct δ1. simpl in *.
+        subst new_cps0 new_eps0.
+        
+        rewrite !mset_filter_difference. 
+        rewrite !mset_filter_singleton.        
+        rewrite filter_union_L.
+        destruct decide.
+        2: { rewrite filter_singleton_not_L; [| tauto].
+             rewrite multiset_difference_empty. rewrite union_empty_r_L.
+             apply ms_le_disj_union.
+             + apply ms_le_sub. reflexivity. 
+             + apply ms_le_exp_le. lia. }
+
+        rewrite filter_singleton_L; [| tauto]. 
+
+        rewrite mset_map_sub_diff. 
+        2: { apply gmultiset_singleton_subseteq_l.
+             by apply mset_filter_spec. }
+        rewrite mset_map_singleton. simpl.
+
+        destruct (decide ((x, x0, x2) ∈ ps_eps)).
+        { rewrite union_comm_L subseteq_union_1_L; [| set_solver].
+          apply ms_le_disj_union.
+          + apply ms_le_sub. mss. 
+          + apply ms_le_exp_le. lia. }
+        
+        forward eapply (approx_expects_add (S k)) as ->.
+        { by intros [??]%elem_of_filter. } 
+        rewrite (gmultiset_disj_union_comm _ ((_ - _) *: _)) gmultiset_disj_union_assoc. 
+        apply ms_le_disj_union; revgoals. 
+        + apply ms_le_exp_le. lia. 
+        + simpl. apply ms_le_exchange.
+          * admit.
+          * eapply elem_of_mset_map. eexists (_, _). split; eauto.
+            apply mset_filter_spec. split; eauto. 
+          * admit.
+    Admitted. 
+
+
+    Lemma other_loc_step_ms_le π__ow δ1 τ δ2 k
+      (STEP: loc_step OP δ1 τ δ2)
+      (OTHER:
+        let π := default π0 (ps_phases _ δ1 !! τ) in
+        phases_incompat π__ow π):
+      ms_le deg_le (PF π__ow (S k) δ2) (PF π__ow k δ1).
+    Proof using.
+      clear sig_le SIG_WF. 
+      rewrite /PF.
+      apply loc_step_split in STEP as [NOEXP | EXP].
+      { eapply loc_step_no_exp_all_ms_le; eauto. }
+      destruct EXP as (?&?&?&T). inversion T; subst.
+      destruct δ1. simpl in *.
+      subst new_cps0.
+      
+      rewrite !mset_filter_disj_union mset_map_disj_union.
+      rewrite !mset_filter_singleton.
+      rewrite decide_False.
+      2: { rewrite LOC_PHASE in OTHER. simpl in OTHER.
+           red in OTHER. tauto. }
+      
+      rewrite mset_map_empty. apply ms_le_disj_union.
+      + eapply ms_le_Proper; [reflexivity| | reflexivity]. mss.
+      + apply ms_le_exp_le. lia. 
+    Qed.
+
+    (* TODO: rename never_set_after *)
+      
+    Lemma min_owner_loc_step_ms_le δ1 τ δ2 k (* s l *)
+      (STEP: loc_step OP δ1 τ δ2)
+      (SET_BOUND: forall sid π d, expects_ep OP δ1 τ δ2 sid π d ->
+                  let n := 2 * (LIM_STEPS + 2) * set_before sid in
+                  k < n)
+      :
+      let π__ow := default π0 (ps_phases _ δ1 !! τ) in
+      ms_le deg_le (PF π__ow (S k) δ2) (PF π__ow k δ1).
+    Proof using.
+      clear sig_le SIG_WF. 
+      rewrite /PF.
+      apply loc_step_split in STEP as [NOEXP | EXP].
+      { eapply loc_step_no_exp_all_ms_le; eauto. }
+
+      destruct EXP as (?&?&?&T). inversion T; subst.
+      destruct δ1. simpl in *.
+      subst new_cps0. rewrite LOC_PHASE. simpl. 
+      
+      rewrite !mset_filter_disj_union mset_map_disj_union.
+      rewrite !mset_filter_singleton.
+      rewrite decide_True; [| reflexivity]. rewrite mset_map_singleton. simpl. 
+
+      (* rewrite mset_map_disj_union. *)
+      rewrite -gmultiset_disj_union_assoc. apply ms_le_disj_union.
+      { apply ms_le_refl. }
+      rewrite (union_difference_singleton_L _ _ EP).
+      
+      rewrite filter_union_L.
+      rewrite !gset_singleton_if_equiv.
+      rewrite decide_True; [| tauto].
+      
+      rewrite (union_comm_L {[ _ ]} _).
+      rewrite !approx_expects_add.
+      2, 3: set_solver.
+      simpl. rewrite gmultiset_disj_union_comm.
+      rewrite -gmultiset_disj_union_assoc.
+      apply ms_le_disj_union.
+      { apply ms_le_exp_le. lia. }
+
+      move SET_BOUND at bottom. specialize_full SET_BOUND; [by eauto| ].
+      eapply ms_le_Proper; [reflexivity| ..| apply ms_le_refl].
+      rewrite -gmultiset_scalar_mul_S_r. f_equiv. lia.
+    Qed.
+
+    Hypothesis (SET_BEFORE_SPEC: 
+                 forall sid i,
+                   (forall c, ¬ never_set_after sid c) ->
+                   set_before sid <= i ->
+                   from_option (fun δ => from_option snd false (ps_sigs _ δ !! sid)) false (tr S!! i) = true).
+
+    (* TODO: move *)
+    Lemma strict_not_both {A: Type} (R: relation A) x y:
+      strict R x y -> strict R y x -> False.
+    Proof using.      
+      clear. intros [??] [??]. done.
+    Qed.
+
+    Lemma tr_loc_step_nsteps_ms_le δ i τ δ' s k
+      (ITH: tr S!! i = Some δ)
+      (BOUND : k ≤ LIM_STEPS)
+
+      (NEVER_SET : never_set_after s i)
+      (MIN: minimal_in_prop tr_sig_lt (s, i)
+          (λ ab : SignalId * nat, never_set_after ab.1 ab.2))
+
+      (OWNER: s ∈ default ∅ (ps_obls _ δ !! τ))
+
+      (STEPS: nsteps (λ p1 p2, loc_step OP p1 τ p2) k δ δ'):
+      let π__ow := default π0 (ps_phases _ δ !! τ) in
+      ms_le deg_le (PF π__ow (2 * (LIM_STEPS + 2) * i + k) δ') (PF π__ow (2 * (LIM_STEPS + 2) * i) δ).
+    Proof using.
+      generalize dependent δ'.
+      induction k.
+      { intros ? ->%obls_utils.nsteps_0.
+        rewrite Nat.add_0_r. reflexivity. }
+      intros δ'' (δ' & STEPS & STEP)%nsteps_inv_r.
+      specialize (IHk ltac:(lia) _ STEPS).
+      etrans; eauto.
+
+      (* follows from well-formedness of state *)
+      assert (ps_phases OP δ !! τ = Some π__ow) as PH by admit. rewrite PH. simpl. 
+      (* follows from preservation of phases before fork *)
+      assert (ps_phases OP δ' !! τ = Some π__ow) as PH' by admit. 
+      
+      eapply ms_le_Proper; [| | eapply min_owner_loc_step_ms_le]; eauto.
+      { rewrite PH'.
+        rewrite -PeanoNat.Nat.add_succ_comm. simpl. reflexivity. }
+      { rewrite PH'. simpl. reflexivity. }
+
+      intros sid π d EXP. simpl.
+      inversion EXP. subst.
+      rewrite PH' in LOC_PHASE. inversion LOC_PHASE. subst π__max.
+      red in OBLS_LT. red in OBLS_LT.
+
+      move NEVER_SET at bottom. red in NEVER_SET.
+      specialize (NEVER_SET _ ltac:(reflexivity)).
+      rewrite ITH in NEVER_SET. simpl in NEVER_SET. 
+      destruct (ps_sigs OP δ !! s) as [[ls ?]|] eqn:SIG__min; [| done].
+      simpl in NEVER_SET. subst. 
+      
+      assert (ps_sigs _ δ' !! s = Some (ls, false)) as SIG' by admit.
+      assert (s ∈ default ∅ (ps_obls _ δ' !! τ)) as OBL' by admit.
+      specialize (OBLS_LT ls). specialize_full OBLS_LT.
+      { apply extract_Somes_gset_spec.
+        destruct (ps_obls OP δ' !! τ) as [obs| ] eqn:OBLS'; [| set_solver].
+        simpl in OBL'. simpl. apply elem_of_map. eexists. split; eauto.
+        rewrite SIG'. done. }
+      assert (strict sig_le l ls) as SIG_LT by admit. clear OBLS_LT.
+
+      enough (set_before sid > i).
+      { apply PeanoNat.Nat.le_succ_l in H0. 
+        apply Nat.le_sum in H0 as [u EQ]. rewrite EQ. lia. }
+      red. destruct (Nat.lt_ge_cases i (set_before sid)) as [?|GE]; [done| ].   
+
+      (* either it was there when the big step started,
+         or it's a new signal, but then the thread holds an obligation
+         and cannot wait on it *)
+      assert (ps_sigs OP δ !! sid = Some (l, false)) as SIG0 by admit.
+
+      pose proof (SET_BEFORE_SPEC sid i). specialize_full H0; [| done| ].
+      2: { rewrite ITH in H0. simpl in H0.
+           rewrite SIG0 in H0. done. }
+
+      intros c NEVER_SET_.
+      assert (never_set_after sid i) as NEVER_SET' by admit. clear NEVER_SET_.
+      move MIN at bottom. red in MIN. specialize (MIN (_, _) NEVER_SET').
+      rewrite /tr_sig_lt /MR in MIN. simpl in MIN.
+      rewrite ITH in MIN. simpl in MIN. rewrite SIG0 SIG__min in MIN. simpl in MIN.
+      specialize (MIN SIG_LT).
+      edestruct @strict_not_both; eauto. 
+    Admitted.
+
+    Theorem signals_eventually_set:
+      ¬ exists sid c, never_set_after sid c. 
+    Proof using.
+      intros EX. apply ex_prod' in EX.
+      eapply sets_have_min in EX; [| apply tr_sig_lt_wf].
+      apply ex_prod in EX. simpl in EX. destruct EX as (s & c & UNSET & MIN).
+      assert (τ__def: Locale) by admit.
+      set (s_ow (i: nat) :=
+             let owners := 
+               dom $ filter (fun '(_, obls) => s ∈ obls)
+               (from_option (ps_obls OP) ∅ (tr S!! i)) in
+             default τ__def (gset_pick owners)
+          ).
+
+      set (OTF i := LTF (s_ow i) i).
+
+      enough (exists d, c <= d /\ OTF d = ∅) as (d & LE & EMP). 
+      { 
+      
+
+      
+
+      
+
+  End SignalsEventuallySet.
 
 
   Section NoInfExpects.
@@ -415,15 +922,6 @@ Section Termination.
 
     Context (deg_le: relation Degree).
 
-    (* TODO: move *)
-    Lemma scalar_mul_le `{Countable K} (s: gmultiset K) m n
-      (LE: m <= n):
-      m *: s ⊆ n *: s.
-    Proof using.
-      clear -LE. 
-      apply Nat.le_sum in LE as [d ->]. multiset_solver.
-    Qed.
-
     (* Lemma approx_expects_next k eps: *)
     (*   approx_expects k eps = ∅ \/ *)
     (*   let add := [^op set] ep ∈ eps, let '(sid, π, d) := ep in {[+ ((* π,  *)d) +]} in *)
@@ -449,6 +947,16 @@ Section Termination.
       apply ms_le_sub.
       apply scalar_mul_le. lia.
     Qed.
+
+    Lemma ms_le_PF_le m n δ
+      (LE: m <= n):
+      ms_le deg_le (PF' n δ) (PF' m δ).
+    Proof using.
+      rewrite /PF'. 
+      apply ms_le_disj_union.
+      + reflexivity.
+      + apply ms_le_exp_le. lia.
+    Qed. 
 
     Lemma approx_expects_add k eps e 
       (FRESH: e ∉ eps):
@@ -566,7 +1074,67 @@ Section Termination.
       + apply ms_le_sub. apply mset_map_sub. mss. 
       + apply ms_le_exp_le. lia.
     Qed.      
- 
+
+    Lemma loc_step_has_exp sid δ1 τ δ2
+      (STEP: loc_step OP δ1 τ δ2)
+      (NO_NOEXP: ¬ loc_step_no_exp sid δ1 τ δ2):
+      exists π d, expects_ep OP δ1 τ δ2 sid π d.
+    Proof using.
+      rewrite /loc_step_no_exp in NO_NOEXP.
+      apply Classical_Prop.not_and_or in NO_NOEXP as [? | EXP]; [tauto| ].
+      apply not_forall_exists_not in EXP as [? EXP].
+      apply not_forall_exists_not in EXP as [? EXP].
+      apply NNP_P in EXP. eauto.
+    Qed.
+
+    From trillium.fairness.lawyer.obligations Require Import obls_utils.
+    Notation " x ;;; y " := (rel_compose x y) (at level 20).
+
+    Definition rep_no_exp n sid ps1 (θ: Locale) ps2 :=
+      relations.nsteps (fun p1 p2 => loc_step_no_exp sid p1 θ p2) n ps1 ps2. 
+
+    Definition progress_step_no_exp sid ps1 (θ: Locale) ps2 :=
+    exists n, n <= LIM_STEPS /\
+           ((* relations.nsteps (fun p1 p2 => loc_step_no_exp sid p1 θ p2) n *)
+             (fun p1 p2 => rep_no_exp n sid p1 θ p2)
+             ;;;
+            (fun p1 p2 => exists π δ, burns_cp OP p1 θ p2 π δ)
+           )
+            ps1 ps2.
+
+    Lemma progres_step_has_exp sid ps1 (θ: Locale) ps2
+      (STEP: progress_step OP ps1 θ ps2)
+      (NO_NOEXP: ¬ progress_step_no_exp sid ps1 (θ: Locale) ps2):
+      False.
+    Proof using.
+      red in STEP. destruct STEP as (n & BOUND & (δ' & PSTEP & BSTEP)).
+      assert (¬ rep_no_exp n sid ps1 (θ: Locale) δ').
+      { intros ?. apply NO_NOEXP. red. eexists. split; eauto.
+        destruct BSTEP as (?&?&?). 
+        eexists. split; eauto. }
+
+      clear -PSTEP H0. 
+
+      
+
+    Lemma tr_loc_step_nsteps_ms_le δ i τ δ' k
+      (ITH: tr S!! i = Some δ)
+      (BOUND : k ≤ LIM_STEPS)
+      (STEPS: nsteps (λ p1 p2, loc_step OP p1 τ p2) k δ δ'):
+  ms_le deg_le (PF' ((LIM_STEPS + 2) * i + k) δ') (PF' ((LIM_STEPS + 2) * i) δ).
+    Proof using.
+      generalize dependent δ'.
+      induction k.
+      { intros ? ->%obls_utils.nsteps_0.
+        rewrite Nat.add_0_r. reflexivity. }
+      intros δ'' (δ' & STEPS & STEP)%nsteps_inv_r.
+      specialize (IHk ltac:(lia) _ STEPS).
+      etrans; eauto.
+      eapply ms_le_Proper; [| reflexivity| eapply locx_step_decr]; eauto.
+      { f_equiv. apply leibniz_equiv_iff. lia. }
+      minimal
+
+
     Lemma step_decr i
       (VALID: obls_trace_valid OP tr):
       ms_lt deg_le (PF (S i)) (PF i).
@@ -612,6 +1180,9 @@ Section Termination.
         f_equiv. apply leibniz_equiv_iff. lia. }
       clear BSTEP.
 
+      etrans.
+      { eapply ms_le_PF_le with (m := (LIM_STEPS + 2) * i + k). lia. }
+      clear dependent 
       
     
    
